Challenge/Ripemd160/Submission/Proofs/Bytecode/StaggerRawPaired16Raw.lean
@@ -20,7 +20,7 @@ def template : List Instr :=
     .op (.Swap ⟨7, by decide⟩),
     .op (.Dup ⟨5, by decide⟩),
     .op (.Dup ⟨10, by decide⟩),
-    .op (.Dup ⟨1, by decide⟩),
+    .op (.Dup ⟨7, by decide⟩),
     .op .OR,
     .op (.Dup ⟨8, by decide⟩),
     .op (.Dup ⟨7, by decide⟩),
